\section{Question 16 \texorpdfstring{$\checkmark$}{\text{âœ“}}}
\horz
Let $V$ be a finite dimensional inner product space with inner product $\langle\cdot ,\cdot \rangle.$ Suppose $\beta_b= (b_1,b_2,\ldots,b_n)$ and  $\beta_e=(e_1,e_2,\ldots,e_n)$ are two ordered basis for $V$ which are related by the following relation:
$e_ j= \sum_{k=1}^n P_{k,j}b_k,$ for $j=1,2,\ldots,n.$ In short (in matrix multiplication notation) they are related by the following :
\begin{align*} \label{Basis change matrix}
(e_1,e_2,\ldots,e_n)= (b_1,b_2,\ldots,b_n)\begin{pmatrix}
P_{1,1} & P_{1,2}& \ldots & P_{1,n}\\
P_{2,1} & P_{2,2}& \ldots & P_{2,n}\\
\vdots & \vdots & \ddots & \vdots\\
P_{n,1} & P_{n,2}& \ldots & P_{n,n}
\end{pmatrix},  \,\,\mbox{that is,}\,\,\beta_e=\beta_b P.
%\,\,P= \begin{pmatrix}
%P_{1,1} & P_{1,2}& \ldots & P_{1,n}\\
%P_{2,1} & P_{2,2}& \ldots & P_{2,n}\\
%\vdots & \vdots & \ddots & \vdots\\
%P_{n,1} & P_{n,2}& \ldots & P_{n,n}
%\end{pmatrix},
\end{align*}
Let $G_e$ and $G_b$  be the Grammian matrix given by 
\begin{align*}
G_e= \begin{pmatrix}
\langle e_1,e_1\rangle & \langle e_2,e_1\rangle & \ldots & \langle e_n,e_1\rangle\\
\langle e_1,e_2\rangle & \langle e_2,e_2\rangle & \ldots & \langle e_n,e_2\rangle\\
\vdots & \vdots & \ddots & \vdots\\
\langle e_1,e_n\rangle & \langle e_2,e_n\rangle & \ldots & \langle e_n,e_n\rangle
\end{pmatrix}, \,G_b= \begin{pmatrix}
\langle b_1,b_1\rangle & \langle b_2,b_1\rangle & \ldots & \langle b_n,b_1\rangle\\
\langle b_1,b_2\rangle & \langle b_2,b_2\rangle & \ldots & \langle b_n,b_2\rangle\\
\vdots & \vdots & \ddots & \vdots\\
\langle b_1,b_n\rangle & \langle b_2,b_n\rangle & \ldots & \langle b_n,b_n\rangle
\end{pmatrix}
\end{align*}
(a) Show that  $G_e = {\bar{P}}^tG_bP,$ where $P$ is the matrix $(\!( P_{i,j})\!).$\\
(b) Show that the matrix $G_b$ is positive definite, that is, 
\begin{itemize}
\item[(i)] ${\bar{G_b}}^t= G_b,$ that is, $G_b$ is self adjoint,
\item[(ii)] $\langle G_b x,x\rangle_2 > 0$ for every non zero $x\in \mathbb C^n.$ Here $\langle\cdot,\cdot\rangle_2 $ denotes the standard Eucledian inner product on $\mathbb C^n.$
\end{itemize}
(c) Show that $\{e_1,e_2,\ldots,e_n\}$ is an orthonormal basis of $V$ if and only if $P {\bar{P}}^t={G_b}^{-1}.$\\
(d) Let $T$ be a linear map from $V$ into itself. Suppose the matrix representation of the linear map $T$ w.r.t the basis $\beta_b$ and $\beta_e$ is given by $[T]_{\beta_b}$
and $[T]_{\beta_e}$ respectively. Show that 
\begin{align*}
[T]_{\beta_e} = [T]_{{\beta_b}P} = P^{-1}[T]_{\beta_b} P.
\end{align*}
\horz

\begin{proof}[Solution]
    \begin{enumerate}[label=(\alph*)]
	\item Let $G_e$ and $G_b$ be the matrix whose entries are given by
   \begin{align*}
       \left( G_{e} \right)_{ij} = \ip{e_{j}, e_{i}}
   \end{align*}
   and 
   \begin{align*}
       \left( G_{b} \right)_{ij} = \ip{b_{j}, b_{i}}
   \end{align*}
   for each $i,j \in \left\{ 1,2,\ldots , n \right\}$.
   Consider the following:
   \begin{align*}
       \left( G_{e} \right) _{ij} &= \ip{e_{j}, e_{i}}  \\
       &= \ip{\sum_{k=1}^{n} P_{kj} b_{k}, \sum_{l=1}^{n} P_{li} b_{l}} \\
       &= \sum_{k=1}^{n} \sum_{l=1}^{n} P_{kj} \ip{b_{k}, b_{l}} \overline{P_{li}} \\
       &= \sum_{k=1}^{n} \sum_{l=1}^{n} \left( P^{*} \right)_{il} (G_{b} )_{lk} P_{kj} \\
       &= \left( P^{*} G_{b} P \right)_{ij}
   \end{align*}
   \item Clearly, we have that 
       \begin{align*}
	   \left( G_{e} ^{*} \right)_{ij} &= \left( \overline{G_{e}} \right) _{ji} \\
	   &= \overline{\ip{e_{i}, e_{j}}} \\
       &= \ip{e_{j}, e_{i}} \\
	   &=  \left( G_{e} \right)_{ij}
       \end{align*}
       for all $i,j$. Hence $G_{e}$ is self-adjoint. Observe that
       \begin{equation*}
	   \ip{G_{b} e_{j} , e_{i}}_{2} = \ip {b_{j}, b_{i}}
       \end{equation*}
       for all $i,j$. Now let $x\in V$. Then there exists unique $x_{1}, x_{2}, \ldots , x_{n}  \in \C$ such that
       \begin{align*}
	   x= \sum_{i=1}^{n} x_{i}e_{i}
       \end{align*}
        Then we have that
	\begin{align*}
	    \ip{G_{b} x , x}_{2} &= \ip{G_{b} \left( \sum_{j=1}^{n}  x_{j} e_{j}  \right), \sum_{i=1}^{n} x_{i} e_{i}} \\
	    &= \sum_{j=1}^{n} \sum_{i=1}^{n} x_{j}\overline{x_{i}} \ip{G_{b} e_{j}, e_{i}} \\
	    &= \sum_{j=1}^{n} \sum_{i=1}^{n} x_{j}\overline{x_{i}} \ip{b_{j}, b_{i}} \\
	    &= \ip{\sum_{j=1}^{n} x_{j} b_{j}, \sum_{i=1}^{n} x_{i} b_{i}}  \\
	    & \ge 0
	\end{align*}
	\item By definition we have that $G_{e} = I$ iff $\left\{ e_{1}, \ldots , e_{n} \right\}$ is orthonormal. ALso from item (a) we have that 
	    \begin{align*}
		\text{$\left\{ e_1 , e_2 , \ldots , e_{n}\right\}$ is orthonormal } &\Leftrightarrow I=P^{*} G_{b} P \\
		& \Leftrightarrow \left( P^{*} \right)^{-1} P^{-1} = G_{b} \\
		& \Leftrightarrow \left( PP^{*} \right)^{-1} G_{b} \\ 
		& \Leftrightarrow PP^{*} = G_{b}^{-1}
	    \end{align*}
	\item Clearly, $P = \left( I \right)_{\beta_{e}}^{\beta ^{b}}$. Then
	    \begin{align*}
		P \left( T \right)_{\beta_{e}} &=  \left( I \right)_{\beta^{e}} ^{\beta_{e}} \\
		&=  \left( I \circ T \right) _{\beta_{e}}^{\beta^{b}} \\
		&= \left( T \circ I \right) _{\beta_{e}}^{\beta^{b}} \\
		&= \left( T \right)_{\beta_{b}}^{\beta_{b}} \left( I \right)_{\beta_{e}}^{\beta_{b}} \\
		&= \left( T \right)_{\beta_{b}} P
	    \end{align*}
	    Hence, we have that 
	    \begin{equation*}
		\left( T \right)_{\beta_e} = P^{-1} \left( T \right)_{\beta_{b}} P
	    \end{equation*}
   \end{enumerate}
   This completes the proof.
\end{proof}
